src/rocq/lib/BvUtil.v
@@ -212,6 +212,13 @@ Qed.
 Definition bv_cast {n m : N} (E : n = m) (x : bv n) : bv m.
 Proof. rewrite E in x. exact x. Defined.
 
+Lemma bv_cast_unsigned : ∀ {n m} {x : bv n} (H : n = m), bv_unsigned (bv_cast H x) = bv_unsigned x.
+Proof. intros ??? H. unfold bv_cast. rewrite <- H. reflexivity. Qed.
+
+Lemma bv_cast_bits {n m : N} (H : n = m) (z : bv n) :
+  bv_to_bits (bv_cast H z) = bv_to_bits z.
+Proof. destruct H. reflexivity. Qed.
+
 Module BoolList.
   (** Convert a list of booleans into a stdpp bitvector. The
   [bits_to_N] function does this by converting the boolean list into a
@@ -224,6 +231,8 @@ Module BoolList.
 
   This seems like the most natural way to do it as it avoids any kind
   of list reversal when converting to the Rocq BinNums-based types. *)
+
+  Open Scope Z_scope.
 
   Definition add_lsb (b : bool) (prefix : option positive) : option positive :=
     match b with
@@ -274,10 +283,141 @@ Module BoolList.
     | Some p => Pos.size_nat p
     end.
 
+  Definition prefix_to_Z (prefix : option positive) : Z :=
+    match prefix with
+    | None => Z0
+    | Some p => Zpos p
+    end.
+
+  Lemma pos_shift_1 : ∀ {p}, Z.pos p ≪ 1 = Z.pos p~0.
+  Proof.
+    intros p.
+    rewrite <- shift_equiv.
+    - reflexivity.
+    - lia.
+  Qed.
+
+  Lemma pos_app_1 : ∀ {p}, Z.lor (Z.pos p ≪ 1) 1 = Z.pos p~1.
+  Proof.
+    intros p.
+    rewrite <- shift_equiv.
+    - reflexivity.
+    - lia.
+  Qed.
+
+  Lemma Z_shiftl_1 : ∀ {x}, x ≪ 1 = 2 * x.
+  Proof. intros. rewrite Z.shiftl_mul_pow2; lia. Qed.
+
+  Lemma Z_shiftl_S : ∀ {x n}, x ≪ Z.of_nat (S n) = (x ≪ 1) ≪ Z.of_nat n.
+  Proof.
+    intros x n.
+    rewrite Z.shiftl_shiftl; [| lia ].
+    f_equal. lia.
+  Qed.
+
+  Lemma Z_shiftl_add_distr : ∀ {a b n}, 0 ≤ n → (a ≪ n) + (b ≪ n) = (a + b) ≪ n.
+  Proof.
+    intros a b n H.
+    repeat rewrite (Z.shiftl_mul_pow2 _ _ H).
+    rewrite Z.mul_add_distr_r.
+    reflexivity.
+  Qed.
+
+  Lemma Z_lor_shift_inc : ∀ {x}, (0 ≤ x)%Z → Z.lor (x ≪ 1) 1 = (x ≪ 1 + 1)%Z.
+  Proof.
+    intros x nonneg.
+    destruct x.
+    - rewrite Z_shiftl_1, Z.mul_0_r, Z.lor_0_l. lia.
+    - rewrite pos_app_1, Z_shiftl_1. lia.
+    - lia.
+  Qed.
+
+  Lemma Z_lor_even : ∀ {x b}, 0 ≤ x → Z.lor (2 * x) (bool_to_Z b) = 2 * x + bool_to_Z b.
+  Proof.
+    intros x b H.
+    destruct x, b; try reflexivity.
+    lia.
+  Qed.
+
+  Lemma Z_mod_even_add_1 (a n : Z) (Ha : 0 ≤ a) (Hn : n > 0) (Heven : (2 | n)%Z) :
+    (2 * a) mod n + 1 = (2 * a + 1) mod n.
+  Proof.
+    destruct Heven as [k Hk].
+    rewrite Z.mul_comm in Hk.
+    subst.
+    rewrite Z.add_mul_mod_distr_l, Z.mul_mod_distr_l.
+    reflexivity.
+    all: try lia.
+  Qed.
+
+  Lemma lsb_prefix_to_Z : ∀ {x p}, prefix_to_Z (add_lsb x p) = prefix_to_Z p ≪ 1 + bool_to_Z x.
+  Proof.
+    intros x p.
+    destruct x, p; cbn.
+    - rewrite <- shift_equiv, Pos2Z.add_pos_pos; [ reflexivity | lia ].
+    - reflexivity.
+    - rewrite <- pos_shift_1, Z.add_0_r. reflexivity.
+    - reflexivity.
+  Qed.
+
+  Lemma to_Z_unsigned_cons : ∀ {x xs p}, to_Z_unsigned (x :: xs) p = to_Z_unsigned xs (add_lsb x p).
+  Proof. intros. reflexivity. Qed.
+
+  Lemma to_Z_unsigned_app_false : ∀ {xs p}, to_Z_unsigned (xs ++ [false]) p = to_Z_unsigned xs p ≪ 1.
+  Proof.
+    intros xs.
+    induction xs as [| x xs IH]; intros p.
+    - destruct p; cbn.
+      + rewrite pos_shift_1. reflexivity.
+      + rewrite Z.shiftl_0_l. reflexivity.
+    - rewrite <- app_comm_cons.
+      rewrite to_Z_unsigned_cons, to_Z_unsigned_cons, IH.
+      reflexivity.
+  Qed.
+
+  Lemma to_Z_unsigned_app_true : ∀ {x p}, to_Z_unsigned (x ++ [true]) p = Z.lor (to_Z_unsigned x p ≪ 1) 1.
+  Proof.
+    intros xs.
+    induction xs as [| x xs IH]; intros p.
+    - destruct p; cbn.
+      + rewrite pos_app_1. reflexivity.
+      + rewrite Z.shiftl_0_l, Z.lor_0_l. reflexivity.
+    - rewrite <- app_comm_cons.
+      rewrite to_Z_unsigned_cons, to_Z_unsigned_cons, IH.
+      reflexivity.
+  Qed.
+
+  Lemma to_Z_unsigned_app : ∀ {x b p}, to_Z_unsigned (x ++ [b]) p = Z.lor (to_Z_unsigned x p ≪ 1) (bool_to_Z b).
+  Proof.
+    intros x b p.
+    destruct b.
+    - rewrite to_Z_unsigned_app_true. reflexivity.
+    - rewrite to_Z_unsigned_app_false. rewrite Z.lor_0_r. reflexivity.
+  Qed.
+
+  Lemma to_Z_unsigned_nil : ∀ {p}, to_Z_unsigned [] p = prefix_to_Z p.
+  Proof. intros. destruct p as [? |]; reflexivity. Qed.
+
+  Lemma to_Z_unsigned_split : ∀ {x p}, to_Z_unsigned x p = prefix_to_Z p ≪ Z.of_nat (length x) + to_Z_unsigned x None.
+  Proof.
+    intros xs.
+    induction xs as [| x xs IH]; intros p; cbn.
+    - rewrite to_Z_unsigned_nil, Z.shiftl_0_r, Z.add_0_r.
+      reflexivity.
+    - rewrite to_Z_unsigned_cons, to_Z_unsigned_cons, (IH (add_lsb x p)), (IH (add_lsb x None)).
+      rewrite lsb_prefix_to_Z, lsb_prefix_to_Z.
+      cbn. rewrite Z.shiftl_0_l, Z.add_0_l, Z_shiftl_1, Z_shiftl_S, Z_shiftl_1, Z.add_assoc, Z_shiftl_add_distr.
+      + reflexivity.
+      + lia.
+  Qed.
+
+  Lemma to_Z_unsigned_nonneg : ∀ x p, 0 ≤ to_Z_unsigned x p.
+  Proof. intros. unfold to_Z_unsigned. destruct_match; lia. Qed.
+
   Lemma Z_pos_size_nat : ∀ {p}, Z.of_N (N.of_nat (Pos.size_nat p)) = Z.pos (Pos.size p).
   Proof. intros p; induction p; cbn; lia. Qed.
 
-  Lemma pow2_pos_size : ∀ {p}, (Z.pos p < 2 ^ Z.pos (Pos.size p))%Z.
+  Lemma pow2_pos_size : ∀ {p}, Z.pos p < 2 ^ Z.pos (Pos.size p).
   Proof.
     intros p.
     rewrite Z.log2_lt_pow2; [| lia].
@@ -285,7 +425,7 @@ Module BoolList.
   Qed.
 
   Lemma to_Z_unsiged_bv_modulus : ∀ {x} prefix,
-    (to_Z_unsigned x prefix < bv_modulus (N.of_nat (prefix_size prefix + length x)))%Z.
+    to_Z_unsigned x prefix < bv_modulus (N.of_nat (prefix_size prefix + length x)).
   Proof.
     intros x.
     induction x as [| [] x IH]; intros prefix.
@@ -324,16 +464,18 @@ Module BoolList.
 
   Definition to_bv (x : list bool) : bv (N.of_nat (length x)) := to_bv' x None.
 
+  Lemma to_bv_unsigned : ∀ {xs}, bv_unsigned (to_bv xs) = to_Z_unsigned xs None.
+  Proof.
+    intros xs.
+    unfold to_bv, to_bv'.
+    rewrite Z_to_bv_small; [ reflexivity |].
+    split.
+    - unfold to_Z_unsigned. destruct_match; lia.
+    - apply (to_Z_unsiged_bv_modulus None).
+  Qed.
+
   Definition positive_to_bv (p : positive) : bv (N.of_nat (Pos.size_nat p)) :=
     Z_to_bv (N.of_nat (Pos.size_nat p)) (Z.pos p).
-
-  Lemma pos_app_1 : ∀ {p}, Z.lor (Z.pos p ≪ 1) 1 = Z.pos p~1 .
-  Proof.
-    intros p.
-    rewrite <- shift_equiv.
-    - reflexivity.
-    - lia.
-  Qed.
 
   Lemma positive_to_bv_concat_1 : ∀ {p}, positive_to_bv p~1 = bv_concat (N.of_nat (S (Pos.size_nat p))) (positive_to_bv p) (1 : bv 1).
   Proof.
@@ -438,12 +580,223 @@ Module BoolList.
           *** apply (Z.lt_le_trans _ _ _ (to_Z_unsiged_bv_modulus None)). reflexivity.
   Qed.
 
-  Lemma bv_round_trip : ∀ {x}, rev (bv_to_bits (to_bv x)) = x.
+  Lemma bv_round_trip_alt : ∀ {x}, bv_to_bits (to_bv x) = rev x.
   Proof.
     intros x.
     unfold to_bv.
     pose proof (@bv_round_trip' x None) as H.
     cbn in H. rewrite H, app_nil_r.
-    apply rev_involutive.
+    reflexivity.
+  Qed.
+
+  Lemma bv_round_trip : ∀ {x}, rev (bv_to_bits (to_bv x)) = x.
+  Proof. intros. rewrite bv_round_trip_alt. apply rev_involutive. Qed.
+
+  Lemma to_bv_ex : ∀ {n} (x : bv n), ∃ y, N.of_nat (length y) = n ∧ ∀ (H : N.of_nat (length y) = n), x = bv_cast H (to_bv y).
+  Proof.
+    intros n x.
+    exists (rev (bv_to_bits x)).
+    split.
+    - simp_length.
+    - intros H.
+      symmetry.
+      apply (inj bv_to_bits).
+      rewrite bv_cast_bits.
+      unfold to_bv.
+      pose proof (@bv_round_trip' (rev (bv_to_bits x)) None) as Hrt.
+      cbn in Hrt. rewrite app_nil_r, rev_involutive in Hrt.
+      exact Hrt.
+  Qed.
+
+  Fixpoint carry_in_rev (c : bool) (xs : list bool) : list bool :=
+    if c then
+      match xs with
+      | [] => [c]
+      | false :: xs => true :: xs
+      | true :: xs => false :: carry_in_rev true xs
+      end
+    else xs.
+
+  Definition carry_in (c : bool) (xs : list bool) : list bool := rev (carry_in_rev c (rev xs)).
+
+  Lemma carry_in_false : ∀ {xs}, carry_in false xs = xs.
+  Proof.
+    intros xs.
+    destruct xs as [| x xs _] using rev_ind.
+    - reflexivity.
+    - unfold carry_in. rewrite rev_unit. cbn. rewrite rev_involutive. reflexivity.
+  Qed.
+
+  Lemma carry_in_to_Z : ∀ {c xs}, to_Z_unsigned (carry_in c xs) None = (to_Z_unsigned xs None + bool_to_Z c)%Z.
+  Proof.
+    intros c xs.
+    revert c.
+    induction xs as [| x xs IH] using rev_ind; intros c.
+    - cbn. destruct_match; cbn; lia.
+    - unfold carry_in. rewrite rev_unit.
+      destruct c, x; cbn; [ fold (carry_in true xs) | | |]; cbn.
+      all: repeat first [ rewrite rev_involutive | rewrite to_Z_unsigned_app_true | rewrite to_Z_unsigned_app_false ].
+      all: try rewrite IH.
+      all: try (repeat rewrite Z_shiftl_1; cbn; lia).
+      all: cbn.
+      + rewrite Z_lor_shift_inc, Z_shiftl_1, Z_shiftl_1; [ lia | apply to_Z_unsigned_nonneg ].
+      + rewrite Z_lor_shift_inc; [ reflexivity | apply to_Z_unsigned_nonneg ].
+  Qed.
+
+  Lemma carry_in_app_true : ∀ {c xs}, carry_in c (xs ++ [true]) = carry_in c xs ++ [xorb c true].
+  Proof.
+    intros c xs.
+    unfold carry_in. rewrite rev_unit.
+    destruct c; cbn [carry_in_rev xorb rev].
+    - reflexivity.
+    - fold (carry_in false xs). rewrite carry_in_false, rev_involutive. reflexivity.
+  Qed.
+
+  Lemma carry_in_app : ∀ {c x xs}, carry_in c (xs ++ [x]) = carry_in (andb c x) xs ++ [xorb c x].
+  Proof.
+    intros c x xs.
+    destruct x.
+    - rewrite andb_true_r. apply carry_in_app_true.
+    - rewrite andb_false_r, carry_in_false.
+      unfold carry_in. rewrite rev_unit.
+      destruct c; cbn [carry_in_rev xorb rev]; rewrite rev_involutive; reflexivity.
+  Qed.
+
+  Lemma to_Z_unsigned_testbit : ∀ {xs i b}, (rev xs) !! i = Some b → Z.testbit (to_Z_unsigned xs None) (Z.of_nat i) = b.
+  Proof.
+    intros xs.
+    induction xs as [| x xs IH] using rev_ind; intros i b H.
+    - cbn in H. rewrite lookup_nil in H. discriminate.
+    - rewrite to_Z_unsigned_app, Z.lor_spec, Z.shiftl_spec; [| lia].
+      destruct i.
+      + rewrite Z.testbit_neg_r, orb_false_l; [| lia].
+        rewrite rev_unit in H. cbn in H. inversion H; subst.
+        rewrite bool_to_Z_spec.
+        assert (D : bool_decide (Z.of_nat 0 = 0%Z) = true).
+        { apply bool_decide_eq_true_2. lia. }
+        rewrite D, andb_true_l.
+        reflexivity.
+      + rewrite bool_to_Z_spec.
+        assert (D: bool_decide (Z.of_nat (S i) = 0%Z) = false).
+        { apply bool_decide_eq_false_2. lia. }
+        rewrite D, andb_false_l, orb_false_r.
+        replace (Z.of_nat (S i) - 1)%Z with (Z.of_nat i); [| lia].
+        rewrite (IH _ b); [ reflexivity |].
+        rewrite <- H, rev_unit, <- lookup_tail.
+        reflexivity.
+  Qed.
+
+  Definition bool_add_carry (x y c : bool) : bool * bool :=
+    match (x, y, c) with
+    | (false, false, false) => (false, false)
+    | (false, false, true ) => (true,  false)
+    | (false, true,  false) => (true,  false)
+    | (false, true,  true ) => (false, true)
+    | (true,  false, false) => (true,  false)
+    | (true,  false, true ) => (false, true)
+    | (true,  true,  false) => (false, true)
+    | (true,  true,  true ) => (true,  true)
+    end.
+
+  Lemma add_carry_step : ∀ {zs} {x y} {xp yp} {z} {in_c out_c},
+    bool_add_carry x y in_c = (z, out_c) →
+    to_Z_unsigned zs None = (prefix_to_Z xp + prefix_to_Z yp)%Z →
+    to_Z_unsigned (carry_in out_c zs ++ [z]) None = (prefix_to_Z (add_lsb x xp) + prefix_to_Z (add_lsb y yp) + bool_to_Z in_c)%Z.
+  Proof.
+    intros zs x y xp yp z c c' Add Tail.
+    destruct z.
+    - rewrite to_Z_unsigned_app_true, carry_in_to_Z, Tail.
+      destruct x, y, c, c', xp, yp; cbn in *; try discriminate.
+      all: try (rewrite Z_lor_shift_inc; [| lia]).
+      all: try rewrite Z_shiftl_1.
+      all: lia.
+    - rewrite to_Z_unsigned_app_false, BoolList.carry_in_to_Z, Tail.
+      destruct x, y, c, c', xp, yp; cbn in *; try discriminate.
+      all: try rewrite BoolList.Z_shiftl_1.
+      all: lia.
+  Qed.
+
+  Fixpoint add_carry_acc (xs ys : list bool) (c : bool) (zs : list bool) : list bool * bool :=
+    match xs with
+    | [] => (zs, c)
+    | x :: xs =>
+        match ys with
+        | [] =>
+            let '(z, c) := bool_add_carry x false c in
+            add_carry_acc xs ys c (z :: zs)
+        | y :: ys =>
+            let '(z, c) := bool_add_carry x y c in
+            add_carry_acc xs ys c (z :: zs)
+        end
+    end.
+
+  Definition add_carry (xs ys : list bool) : list bool * bool :=
+    add_carry_acc (rev xs) (rev ys) false [].
+
+  Lemma add_carry_acc_to_Z : ∀ xs ys c zs,
+    length xs = length ys →
+    to_Z_unsigned (add_carry_acc (rev xs) (rev ys) c zs).1 None =
+      ((to_Z_unsigned xs None + to_Z_unsigned ys None + bool_to_Z c) `mod` 2 ^ Z.of_nat (length xs))
+      ≪ Z.of_nat (length zs) + to_Z_unsigned zs None.
+  Proof.
+    intros xs.
+    induction xs as [| x xs IH] using rev_ind; intros ys c zs L.
+    - assert (ys_nil : ys = []).
+      { apply nil_length_inv. naive_solver. }
+      subst. cbn.
+      rewrite Z.mod_1_r, Z.shiftl_0_l.
+      reflexivity.
+    - rewrite length_app in L. cbn in L. rewrite Nat.add_1_r in L.
+      destruct ys as [| y ys _] using rev_ind; [ discriminate |].
+      rewrite length_app in L; cbn in L. rewrite Nat.add_1_r in L. apply eq_add_S in L.
+      unfold add_carry.
+      repeat rewrite rev_unit.
+      cbn [add_carry_acc].
+      destruct (bool_add_carry x y c) as (z, c') eqn : Add.
+      specialize (IH ys c' (z :: zs) L).
+      rewrite IH.
+      repeat rewrite to_Z_unsigned_app.
+      repeat rewrite Z_shiftl_1, Z_lor_even; try apply to_Z_unsigned_nonneg.
+      cbn [length].
+      rewrite Z_shiftl_S, Z_shiftl_1.
+      rewrite to_Z_unsigned_cons.
+      repeat rewrite Z.add_assoc.
+      rewrite <- Zmult_mod_distr_l.
+      replace (2 ^ Z.of_nat (length (xs ++ [x])))%Z
+        with (2 * 2 ^ Z.of_nat (length xs))%Z; [| shelve ].
+      assert (Lxyc : (bool_to_Z x + bool_to_Z y + bool_to_Z c = bool_to_Z z + 2 * bool_to_Z c')%Z).
+      { destruct x, y, z, c, c'; cbn in Add |- *; discriminate + reflexivity. }
+      repeat rewrite Z.mul_add_distr_l.
+      replace (2 * to_Z_unsigned xs None + bool_to_Z x + 2 * to_Z_unsigned ys None + bool_to_Z y + bool_to_Z c)%Z
+        with (2 * to_Z_unsigned xs None + 2 * to_Z_unsigned ys None + (bool_to_Z x + bool_to_Z y + bool_to_Z c))%Z; [| lia].
+      rewrite Lxyc.
+      repeat rewrite Z.add_assoc.
+      rewrite (@to_Z_unsigned_split zs (add_lsb z None)).
+      rewrite Z.add_assoc, Z_shiftl_add_distr, lsb_prefix_to_Z; [| lia].
+      repeat f_equal.
+      destruct z.
+      + cbn.
+        replace (2 * to_Z_unsigned xs None + 2 * to_Z_unsigned ys None + 1 + 2 * bool_to_Z c')%Z
+          with (2 * (to_Z_unsigned xs None + to_Z_unsigned ys None + bool_to_Z c') + 1)%Z; [| lia].
+        rewrite <- Z_mod_even_add_1; [ repeat f_equal; lia | shelve | lia | apply Z.divide_factor_l ].
+      + cbn. rewrite Z.add_0_r, Z.add_0_r. reflexivity.
+      Unshelve.
+      { rewrite length_app. cbn. rewrite Nat.add_1_r, Nat2Z.inj_succ, Z.pow_succ_r.
+        - reflexivity.
+        - lia. }
+      { apply Z.add_nonneg_nonneg;
+          [ apply Z.add_nonneg_nonneg; apply to_Z_unsigned_nonneg | destruct c'; cbn; lia ]. }
+  Qed.
+
+  Lemma add_carry_to_Z (xs ys : list bool) :
+    length xs = length ys →
+    to_Z_unsigned (add_carry xs ys).1 None =
+      (to_Z_unsigned xs None + to_Z_unsigned ys None) `mod` 2 ^ Z.of_nat (length xs).
+  Proof.
+    intros H.
+    unfold add_carry.
+    rewrite (add_carry_acc_to_Z _ _ _ _ H).
+    cbn. rewrite Z.shiftl_0_r, Z.add_0_r, Z.add_0_r.
+    reflexivity.
   Qed.
 End BoolList.
